proved `valid_pure` and `valid_bind`

Mt/Task/Validation.lean
@@ -8,17 +8,53 @@ local instance : IsReservation spec.Reservation :=spec.is_reservation
 
 def valid {T : Type} (p : TaskM spec T) (r : spec.Reservation)
   (assuming : spec.Reservation -> Bool)
-  (motive : T -> spec.Reservation -> spec.State -> Prop)
+  (motive : T -> spec.Reservation -> Prop)
   : Prop :=∀ env_r s,
     assuming (env_r + r) →
     spec.validate (env_r + r) s →
     match h : p.iterate r s with
-    | IterationResult.Done r' s' t => spec.validate (env_r + r') s' ∧ motive t r' s'
+    | IterationResult.Done r' s' t => spec.validate (env_r + r') s' ∧ motive t r'
     | IterationResult.Panic .. => False
     | IterationResult.Running r' s' block_until cont =>
         spec.validate (env_r + r') s' ∧
         cont.valid r' block_until motive
 termination_by valid => p
 decreasing_by simp_wf ; exact is_direct_cont.running h
+
+theorem valid_pure {T : Type} {t : T} {r assuming motive}
+  (is_valid : motive t r)
+  : valid (spec :=spec) (pure t) r assuming motive :=by
+  rw [valid]
+  intro env_r s _ initial_valid
+  rw [iterate_pure]
+  exact ⟨initial_valid, is_valid⟩
+
+theorem valid_bind {U V : Type}
+  {mu : TaskM spec U}
+  {f : U -> TaskM spec V}
+  {r assuming motive}
+  (motive_u : U -> spec.Reservation -> Prop)
+  (mu_valid : mu.valid r assuming motive_u)
+  (f_valid : ∀ r' u,
+    motive_u u r' →
+    (f u).valid r' (λ _ => true) motive)
+  : valid (mu >>= f) r assuming motive :=by
+  rw [valid]
+  intro env_r s assuming_true initial_valid
+  rw [iterate_bind]
+  rw [valid] at mu_valid
+  cases iteration : iterate mu r s
+  all_goals (
+    simp only []
+    have mu_valid :=mu_valid env_r s assuming_true initial_valid
+    rw [iteration] at mu_valid
+    simp only [] at mu_valid
+  )
+  . exact ⟨mu_valid.left, f_valid _ _ mu_valid.right⟩
+  . constructor
+    . exact mu_valid.left
+    . have :=is_direct_cont.running iteration
+      exact valid_bind motive_u mu_valid.right f_valid
+termination_by valid_bind => mu
 
 end Mt.TaskM
